Cleaner way to perform block-unblocking for instruction search

vale/code/lib/transformers/Vale.Transformers.InstructionReorder.fst
@@ -1577,6 +1577,17 @@ let rec lemma_num_blocks_in_codes_append (c1 c2:codes) :
   | [] -> ()
   | x :: xs -> lemma_num_blocks_in_codes_append xs c2
 
+let rec unblock_once (c : codes) :
+  Pure (possibly codes)
+    (requires True)
+    (ensures (fun r -> Ok? r ==> num_blocks_in_codes c = num_blocks_in_codes (Ok?.v r) + 1)) =
+  match c with
+  | [] -> Err "Cannot unblock further"
+  | Block l :: xs -> Ok (l `L.append` xs)
+  | x :: xs ->
+    xs' <-- unblock_once xs;
+    return (x :: xs')
+
 let rec reordering_allowed (c1 c2 : codes) :
   Tot pbool
     (decreases %[c2; num_blocks_in_codes c1]) =
@@ -1594,10 +1605,12 @@ let rec reordering_allowed (c1 c2 : codes) :
         match h1, h2 with
         | Block l1, Block l2 ->
           reordering_allowed l1 l2 &&. reordering_allowed t1 t2
-        | Block l1, _ -> (
-            reordering_allowed (l1 `L.append` t1) c2
+        | _ -> (
+            match unblock_once c1 with
+            | Ok c1' ->
+              reordering_allowed c1' c2 (* TODO: Handle IfElse and While specially too? *)
+            | Err _ -> Err reason
           )
-        | _ -> Err reason (* TODO: Handle IfElse and While specially too? *)
       )
 
 (** Transform [c1] into the ordering specified by [c2] *)
@@ -1620,8 +1633,8 @@ let rec perform_reordering (c1 c2 : codes) :
         | Block l1, Block l2 ->
           assert (eq_code (Block (perform_reordering l1 l2)) (Block l2)); (* OBSERVE *)
           Block (perform_reordering l1 l2) :: perform_reordering t1 t2
-        | Block l1, _ ->
-          perform_reordering (l1 `L.append` t1) c2
+        | _ ->
+          perform_reordering (Ok?.v (unblock_once c1)) c2
       )
 
 /// If there are two sequences of instructions that can be transformed
@@ -1677,6 +1690,23 @@ let rec lemma_machine_eval_codes_block_to_append (c1 c2 : codes) (fuel:nat) (s:m
       lemma_machine_eval_codes_block_to_append xs c2 fuel s1
 #pop-options
 
+let rec lemma_unblock_once (c : codes) (fuel:nat) (s:machine_state) :
+  Lemma
+    (requires (Ok? (unblock_once c)))
+    (ensures (
+        let Ok c' = unblock_once c in
+        machine_eval_codes c fuel s == machine_eval_codes c' fuel s)) =
+  match c with
+  | Block x :: xs -> (
+      lemma_machine_eval_codes_block_to_append x xs fuel s
+    )
+  | x :: xs -> (
+      match machine_eval_code x fuel s with
+      | None -> ()
+      | Some s1 ->
+        lemma_unblock_once xs fuel s1
+    )
+
 let rec lemma_reordering (c1 c2 : codes) (fuel:nat) (s1 : machine_state) :
   Lemma
     (requires (
@@ -1728,7 +1758,7 @@ let rec lemma_reordering (c1 c2 : codes) (fuel:nat) (s1 : machine_state) :
           assert (equiv_states s2' s2'');
           assert (machine_eval_codes (perform_reordering c1 c2) fuel s1 == machine_eval_codes (perform_reordering t1 t2) fuel s1'');
           assert (Some s2'' == machine_eval_codes (perform_reordering c1 c2) fuel s1)
-        | Block l1, _ ->
-          lemma_machine_eval_codes_block_to_append l1 t1 fuel s1;
-          lemma_reordering (l1 `L.append` t1) c2 fuel s1
+        | _ ->
+          lemma_unblock_once c1 fuel s1;
+          lemma_reordering (Ok?.v (unblock_once c1)) c2 fuel s1
       )
